% !TEX spellcheck = en_US
% !TEX spellcheck = LaTeX
\documentclass[a4paper,10pt,english]{article}
\include{header}
\title{Lecture 12 : Continuous Time Markov Chains}
\author{}
\begin{document}
\maketitle

\section{Axiomatic Definition}
\begin{defn}
A continuous time stochastic process $\{X(t) \in \N_0,~ t \geqslant 0\}$ is a \textbf{continuous time Markov chain (CTMC)} if
\begin{align*}
\Pr\{X(t+s) = j |X(u),~ u \in [0,s]\} &= \Pr\{X(t+s) = j |X(s)\}, \text{ for all } s, t \geqslant 0 \text{ and } i, j \in \N_0.
\end{align*}
We define the \textbf{transition probability} from state $i$ at time $s$ to state $j$ at time $s+t$ as 
\begin{align*}
P_{ij}(s, s+t) = \Pr\{X(s+t) = j | X(s) = i\}.
\end{align*}
The CTMC has \textbf{homogeneous} transitions if $P_{ij}(s,s+t) = P_{ij}(0,t)$ for all $i,j \in \N_0, s,t \geqslant 0$ and we denote the transition probability by $P_{ij}(t)$. 
\end{defn}

\subsection{Sojourn Times and Jump Transitions}
Suppose $X(0)=i$, and  for all $u \in [0,s]$, we have $X(u)=i$. We are interested in knowing probabilities of the form $\Pr\{X(v)=i,~v \in [s,s+t] | X(u)=i, ~ u \in [0,s]\}$. To this end, we define sojourn times in any state.
\begin{defn}
Sojourn times of a CTMC $\{X(t), t \geqslant 0\}$ is defined by
\begin{align*}
\tau_i \triangleq \{t \geqslant 0: X(t) \neq i|X(0)=i\}, i \in \N_0. 
\end{align*}
\end{defn}
\begin{lem}
For a homogeneous CTMC, sojourn time $\tau_i$ is a continuous memoryless random variable. %and exponentially distributed. 
\end{lem}
\begin{proof}
We observe that,
\begin{align*}
\Pr\{\tau_i \geqslant s+t | \tau_i > s\} &=\Pr\{X(v)=i,~v \in [s,s+t) | X(u)=i,  i \in [0, s]\}\\
&= \Pr\{X(v)=i,~v \in [0,t) | X(0)=i\} = \Pr\{\tau_i \geqslant t \}.
\end{align*}
\end{proof}
We could sample the process at these instants and construct a DTMC and study the same. 
\begin{defn}
Jump transition probabilities of a CTMC $\{X(t), t \geqslant 0\}$ are defined by
\begin{align*}
p_{ij} \triangleq \Pr\{X(\tau_i)  = j | X(0) =  i \}, ~i,j \in \N_0.
\end{align*}
\end{defn}
\begin{lem}
For a homogeneous CTMC, jump transition probabilities $p_{ij}$ add to unity for all $i \in \N_0$.
\end{lem}
\begin{proof}
\end{proof}

\subsection{Alternative way of constructing CTMC}
\begin{prop} A continuous time stochastic process $\{X(t) \in \N_0, t \geqslant 0 \}$ is a CTMC iff \begin{enumerate}
\item sojourn time $\tau_i$ is distributed with $\exp(\nu_i)$, and 
\item jump transition probabilities $p_{ij}$ is such that $\sum_{i \neq j}p_{ij}=1$.
\end{enumerate}
\end{prop}
\begin{proof}
\end{proof}
\begin{rem}
Transition probabilities $p_{ij}$ and sojourn times $\tau_i$ are independent. 
\end{rem}
\begin{rem} Inverse of mean sojourn time $\nu_i$ is called rate of state $i$, and typically $\nu_i < \infty$.  
\end{rem}
\begin{rem} If $\nu_i = \infty$, we call the state to be instantaneous. 
\end{rem}
\begin{rem}  A CTMC is a DTMC with exponential sojourn time in each state.
\end{rem}
\begin{defn} A CTMC is called \textbf{regular} if 
\begin{align*}
\Pr\{ \text{ number of transitions in } [0,t] \text{ is finite}\} = 1,~ \forall t < \infty.
\end{align*} 
\end{defn}
\begin{exmp} Consider the following example of a non-regular CTMC. $p_{i,i+1}=1, \nu_i = i^2$. Show that it is not regular.
\end{exmp}

\section{Generator Matrix}
\begin{defn}
A \textbf{generator matrix} denoted by $Q$ is defined in terms of sojourn times $\nu_i$ and jump transition probabilities $p_{ij}$ of a CTMC as
\begin{enumerate}
\item {$q_{ij}=\nu_i p_{ij}$, $\forall i \neq j$, } 
\item { $q_{ii}= -\nu_i$.}
\end{enumerate}
\end{defn}
\begin{lem} Generator matrix $Q$ has following properties.
 \begin{enumerate}
\item {$0 \leq -q_{ii} < \infty,~ \forall i$.} 
\item { $q_{ij} \geq 0,~ \forall i \neq j$.}
\item { $\sum_{j}q_{ij}=0,~ \forall i$.}
\end{enumerate}
\end{lem}

From the $Q$ matrix, we can construct the whole CTMC.  In DTMC, we had the result $P^{(n)}(i,j)=(P^n)_{i,j}$. We can generalize this notion  in the case of CTMC as follows: $P=e^{Q}\triangleq \sum_{k \in \mathbb{N}_0}\frac{Q^k}{k !}$.  Observe that $e^{Q_1+Q_2}=e^{Q_1}e^{Q_2},~ e^{nQ}=(e^Q)^n=P^n$.\\
\begin{thm}
Let $Q$ be a finite sized matrix. Let $\Pr\{t)=e^{tQ}$. Then $\{\Pr\{t),~ t \geq 0\}$ has the following properties:\begin{enumerate}
\item {$\Pr\{s+t)=\Pr\{s)\Pr\{t),~ \forall s,~t$ (semi group property).}
\item {$\Pr\{t),~t \geq 0$ is the unique solution to the forward equation, $\frac{d\Pr\{t)}{dt}=\Pr\{t)Q,~\Pr\{0)=I$.}
\item {And the backward equation $\frac{d\Pr\{t)}{dt}=Q\Pr\{t),~\Pr\{0)=I$.}\\
\item {For all $k \in \mathbb{N}$, $\frac{d^k\Pr\{t)}{d^k(t)}|_{t=0}=Q^k$.}
\end{enumerate}
\end{thm}  
\begin{proof}
$\frac{dM(t)e^{-tQ}}{dt}=0,$ $M(t)e^{-tQ}$ is constant. $M(t)$ is any matrix satisfying the forward equation.
\end{proof}
\begin{thm}
A finite matrix $Q$ is $Q$ matrix if and only if $\Pr\{t)=e^{tQ}$ is a stochastic matrix for all $t \geq 0$. 
\end{thm}
\begin{proof}
$\Pr\{t)=I+tQ+O(t^2)$ ($f(t)=O(t) \Rightarrow \frac{f(t)}{t} \leq c,$ for small $t,~c < \infty$ ). $q_{ij} \geq 0$ if and only if $P_{ij}(t) \geq 0,~ \forall i \neq j$ and $t \geq 0$ sufficiently small. $\Pr\{t)=\Pr\{\frac{t}{n})^n$. Note that if $Q$ has zero row sums, $Q^n$ also has zero row sums.\\
\begin{flalign*}
\sum_j [Q^n]_{ij}&= \sum_j \sum_k [Q^{n-1}]_{ik}Q_{kj}= \sum_j \sum_k Q_{kj}[Q^{n-1}]_{ik}=0.\\
\sum_{j}P_{ij}(t)&=1+\sum_{n \in \mathbb{N}} \frac{t^n}{n!}\sum_j [Q^n]_{ij}=1+0=1.
\end{flalign*}  
Conversely $\sum_{j}P_{ij}(t)=1,~ \forall t \geq 0$, then $\sum_jQ_{ij}= \frac{dP_{ij}(t)}{dt}=0$.
\end{proof}
\subsection{Kolmogorov Differential Equations}
\begin{lem}
\begin{enumerate}
\item{$\lim_{t \rightarrow 0} \frac{1-P_{ii}(t)}{t}=\nu_i$.}\\
\item{$\lim_{t \rightarrow 0} \frac{P_{ij}(t)}{t}=q_{ij}$.}
\end{enumerate}
\end{lem}
\begin{lem}
For all $s,~t \geq 0$, $P_{ij}(t+s)=\sum_{k \in \mathbb{N}_0 P_{ik}(t)P_{kj}(s)}$
\end{lem}
\subsection{Chapman Kolmogorov Equation for CTMC}
\begin{thm}
\textbf{Kolmogorov Backward equation:} For all $i,j,t \geq 0$, $P'_{ij}(t)= \sum_{k \neq i}q_{ik}P_{kj}(t)-\nu_iP_{ij}(t)$ ,  $\frac{d\Pr\{t)}{dt}=Q\Pr\{t)$
\end{thm}
\begin{proof}
$P_{ij}(t+h)=\sum_kP_{ik}(h)P_{kj}(t).$
\begin{flalign*}
P_{ij}(t+h)-P_{ij}(t)=\sum_{k \neq 1}P_{ik}(h)P_{kj}(t)-(1-P_{ii}(h))P_{ij}(t), 
\end{flalign*}
divide by $h$, $h \rightarrow 0$, we get $\frac{dP_{ij}(t)}{dt}=\lim_{h \rightarrow 0}P'_{ij}(t)= \sum_{k \neq i}q_{ik}P_{kj}(t)-\nu_iP_{ij}(t)$. Now the exchange of limit and summation has to be justified. 
\begin{flalign*}
&\liminf_{h \rightarrow 0} \sum_{k \neq 1}\frac{P_{ik}(h)}{h}P_{kj}(t) \geq \liminf_{h \rightarrow 0}\sum_{k \neq 1}\frac{P_{ik}(h)}{h}P_{kj}(t), k <N\\
&= \sum_{k \neq 1}q_{jk}P_{kj}(t),~k <N.
\end{flalign*}
This is true for any finite $N$. Take supremum over all $N$. We get \\
$\liminf_{h \rightarrow 0} \sum_{k \neq 1}\frac{P_{ik}(h)}{h}P_{kj}(t) \geq \sum_{k \neq 1}q_{jk}P_{kj}(t)$. Suffices to show that $\limsup_{h \rightarrow 0} \sum_{k \neq 1}\frac{P_{ik}(h)}{h}P_{kj}(t) \leq \sum_{k \neq 1}q_{jk}P_{kj}(t)$. To that end, 
\begin{flalign*}
\text{LHS}& \leq \limsup_{h \rightarrow 0}[\sum_{k \neq 1, k<N}\frac{P_{ik}(h)}{h}P_{kj}(t)+\sum_{k \neq 1, k\geq N}\frac{P_{ik}(h)}{h} ]\\
& = \limsup_{h \rightarrow 0}[\sum_{k \neq 1, k<N}\frac{P_{ik}(h)}{h}P_{kj}(t)+\frac{1-P_{ii}(h)}{h} \sum_{k \neq 1, k\geq N}\frac{P_{ik}(h)}{h} ]\\
& = [\sum_{k \neq 1, k<N}q_{ik}P_{kj}(t)+\nu_i- \sum_{k \neq 1, k\geq N}q_{ik} ]\\
&=\sum_{k \neq 1}q_{ik}P_{kj}(t). 
\end{flalign*}
\end{proof}
\begin{thm}
\textbf{Kolmogorov Forward Equation:} Under suitablle reqularity conditions, $P'_{ij}(t)=\sum_{k \neq i}P_{ik}(t)q_{kj}-P_{ij}(t)\nu_i$, i.e. $\frac{d\Pr\{t)}{dt}=\Pr\{t)Q$.
\end{thm}
\end{document}
